src/LLBC.v
@@ -133,7 +133,7 @@ Next Obligation.
   - rewrite decode'_is_Some in H.
     destruct s; cbn; rewrite <-H; symmetry;
       first [apply sum_maps_alter_inl | apply sum_maps_alter_inr].
-  - symmetry. apply map_alter_not_in_domain, sum_maps_lookup_None. assumption.
+  - symmetry. apply alter_id', sum_maps_lookup_None. assumption.
 Qed.
 (* What are the two following obligations? *)
 Next Obligation. discriminate. Qed.
@@ -416,9 +416,9 @@ Ltac eval_var :=
   split; [eexists; split; [reflexivity | constructor] | ].
 
 Section Eval_LLBC_program.
-  Hint Rewrite (@alter_insert _ _ _ _ _ _ _ _ _ _ Pmap_finmap) : core.
+  Hint Rewrite (@alter_insert_eq _ _ _ _ _ _ _ _ _ _ Pmap_finmap) : core.
   Hint Rewrite (@alter_insert_ne _ _ _ _ _ _ _ _ _ _ Pmap_finmap) using discriminate : core.
-  Hint Rewrite (@alter_singleton _ _ _ _ _ _ _ _ _ _ Pmap_finmap) : core.
+  Hint Rewrite (@alter_singleton_eq _ _ _ _ _ _ _ _ _ _ Pmap_finmap) : core.
 
   Lemma insert_empty_is_singleton `{FinMap K M} {V} k v : insert (M := M V) k v empty = {[k := v]}.
   Proof. reflexivity. Qed.
